minor edit to the paxos model

paxos-classic.dfy
@@ -1,7 +1,8 @@
 /* We establish a classic paxos model referring to 
  ** the 2001 paper (Leslie Lamport. Paxos Made Simple) and 
  ** the 2004 paper (Jim Gray and Leslie Lamport: Consensus on Transaction Commit. MSR-TR-2003-96)
- * We refer to the original paper of Lamport for a detailed understanding of Paxos if you are confused with part of this model
+ ** the author also consulted this website https://uvdn7.github.io/paxos-explained/ to achieve a better understanding in Paxos
+ * Overall we refer to the original paper of Lamport for a detailed understanding of Paxos if you are confused with part of this model
  * (Leslie Lamport. The part-time parliament. ACM transactions on Computer Systems, 16(2):133-169, May 1998)
  * There are other variants of Paxos, such as Fast Paxos, Byzantine Paxos, and Raft.
  *
@@ -10,21 +11,21 @@
  * - Acceptors: which accept and decide a value under the coordination of (one or more) coordinators
  * - Learners: which learns a value after the protocol reaches a decide phase
  *
- * We assume asynchronous communication model, i.e., messages may not get lost, but there is not a time bound for message delivery
+ * We assume asynchronous communication model, i.e., messages cannot get lost, but there does not exist a time bound for message delivery
  * Integrity/Correctness: a decided value must be proposed by a coordinator
  * Consistency/Safety: a single value is decided (for each protocol round/view/cycle)
  *
  * Note that classic paxos assumes that no participant is malicious. 
- * However, a participant may become faulty, as long as the total number of faulty node is less than half of the total number of nodes.
+ * A participant may become faulty, as long as the total number of faulty node is less than half of the total number of nodes.
  * The total number of nodes is known to everyone.
  * 
  * Simplifications in the model:
- * -- We assume an coordinator picks a ballot when it becomes active (is event is atomic)
- * -- The ballot being selected is ever increasing, starting from 0; Each coordinator's ballot number is unique/distinct
+ * -- We assume that an coordinator picks a ballot when it becomes active (this event is atomic)
+ * -- The ballot number to be selected is ever increasing, starting from 0; This implies every coordinator's ballot number is unique/distinct
  * -- Each time a ballot is picked, such information is broadcast to every acceptor
- * -- A message is recorded in a global data structure, and may be delivered to each individual node by individual action (modelling asynchrony)
+ * -- A message is recorded in a global data structure, and may be delivered to each individual node by an individual "receive" action (modelling asynchrony)
  * -- We assume all messages are broadcast (since no party is malicious)
- * -- No modelling message loss (as it cannot be distinguished from being ignored by the receiver)
+ * -- No modelling message of loss (as it cannot be distinguished from being ignored by the receiver)
  * -- If a node becomes faulty, then its irreversible (unlike a sleepy node in a sleepy model)
  * -- Learners are NOT explicitly modelled. We can directly observe a decision value if a leader/coordinator performs Step 3a.
  * -- We only model a single round of consensus
@@ -44,12 +45,12 @@ lemma{:axiom} Quorum()
 
 // an internal state of an acceptor: the highest ballot so far and its associated value 
 datatype AState = AState(highest: int, value: Proposal) 
+// an internal state of a leader: its ballot and its value to be proposed
+datatype LState = LState(ballot: int, value: Proposal)
 // the message type from an acceptor in step 1b
-datatype AMsg = AMsg(ballot: int, highest: int, value: Proposal, acc: Acceptor)
+datatype PMsg = PMsg(ballot: int, highest: int, value: Proposal, acc: Acceptor)
 // the message type from an acceptor in step 2b
 datatype CMsg = CMsg(ballot: int, value: Proposal, acc: Acceptor)
-// a triple representing a promise from an acceptor in step 1b: current highest promise, highest value, and the acceptor ID
-datatype Promise = Promise(highest: int, value: Proposal, acc: Acceptor)
 
 // a global state of a Paxos protocol run
 datatype TSState = TSState(
@@ -57,17 +58,18 @@ datatype TSState = TSState(
     leader_propose: map<Acceptor, Proposal>,  // updated in step 2a for a leader when it proposes a value, initially 0
     leader_decision: map<Acceptor, Proposal>, // updated in step 3a for a leader when it decides a value, initially 0
     ballot: int,  // initially 0
-    // all states of acceptors
+    // states of acceptors
     acceptor_state: map<Acceptor, AState>,  
-    // counting the response of the form <bal, -1, 0> from any acceptor message in step 1b
-    empty_count: map<Acceptor, set<Acceptor>>, 
-    // counting the response of the form <bal, highest_bal, v> from any acceptor message in step 1b
-    ballot_count: map<Acceptor, set<Promise>>,    
-    // counting response from acceptors <bal, val, acceptor> in step 2b, where the domain of the map is the leader
-    // Here, different leaders making same decision is possible, but his does not affect the checking of consistency/safety.
+    // states of leaders
+    leader_state: map<Acceptor, LState>,  
+    // counting the response of the form <highest_bal, bal, value, acc> from any acceptor message in step 1b
+    // where the domain of the map is the leaders
+    promise_count: map<Acceptor, set<Acceptor>>,    
+    // counting response from acceptors <bal, val, acceptor> in step 2b, where the domain of the map is the leaders
+    // Here, different leaders making same decision is possible, but this should not affect the checking of consistency/safety.
     decision_count: map<Acceptor, set<Acceptor>>,
     // the set of messages sent by acceptors in step 1b
-    amsgs: set<AMsg>,
+    pmsgs: set<PMsg>,
     // the set of messages sent by acceptors in step 2b
     cmsgs: set<CMsg>
 )
@@ -75,11 +77,13 @@ datatype TSState = TSState(
 // define the constraints for the types of a state components
 ghost predicate type_ok(s: TSState){
     && s.leader_ballot.Keys == s.leader_propose.Keys == s.leader_decision.Keys 
-        == s.empty_count.Keys == s.decision_count.Keys == s.ballot_count.Keys == leaders
+        == s.promise_count.Keys == s.decision_count.Keys == leaders
     && s.acceptor_state.Keys == acceptors
+    && s.leader_state.Keys == leaders
     //&& forall n :: n in leaders ==> (forall v :: v in s.ballot_count[n].Keys ==> v >= -1)
 }
 // define what a valid state is in a Paxos run
+// we may also add invariants into this predicate later
 ghost predicate valid(s: TSState){
     true
 }
@@ -95,15 +99,17 @@ ghost predicate init(s: TSState)
     && (forall n :: n in leaders ==> s.leader_decision[n] == 0)
     && (forall n :: n in leaders ==> s.decision_count[n] == {})
     && (forall a :: a in acceptors ==> s.acceptor_state[a] == AState(-1, 0))
-    && (forall n :: n in leaders ==> s.empty_count[n] == {})
-    && (forall n :: n in leaders ==> s.ballot_count[n] == {})
-    && s.amsgs == {} && s.cmsgs == {}
+    && (forall n :: n in leaders ==> s.leader_state[n] == LState(-1, 0))
+    && (forall n :: n in leaders ==> s.promise_count[n] == {})
+    && (forall n :: n in leaders ==> s.decision_count[n] == {})
+    && s.pmsgs == {} && s.cmsgs == {}
 }
 
-// In the following we define each transition relation following the Paxos protocol.
+// In the following we define a transition relation for each step following the Paxos protocol.
 //
 // Step 1a: a leader (coordinator) chooses a ballot number & sends it to every acceptor. 
-// This ballot number may be received by an acceptor sometime later.
+// This ballot number may be received by an acceptor sometime later, 
+// which is modelled by (an acceptor later) looking into the leader_ballot component.
 predicate choose_ballot(s: TSState, s': TSState, c: Acceptor)
   requires type_ok(s) && type_ok(s') && valid(s) && c in leaders
 {
@@ -114,52 +120,52 @@ predicate choose_ballot(s: TSState, s': TSState, c: Acceptor)
     && s'.leader_propose == s.leader_propose
     && s'.leader_decision == s.leader_decision
     && s'.acceptor_state == s.acceptor_state
-    && s'.empty_count == s.empty_count
-    && s'.ballot_count == s.ballot_count
+    && s'.leader_state == s.leader_state
+    && s'.promise_count == s.promise_count
     && s'.decision_count == s.decision_count
 }
-// Step 1b: an acceptor may receive message 1a from a leader (coordinator) ometime later
-// In this case, the ballot number is higher than the acceptor's highest recorded ballot
+// Step 1b: an acceptor may receive message 1a from a leader (coordinator) sometime later
+// In this case, the ballot number is higher than the acceptor's highest recorded ballot.
+// There are two possibilities here: 
+// (1) the acceptor has not yet confirmed any value; 
+// (2) the acceptor has already confirmed some value previously
 predicate receive_higher_ballot(s: TSState, s': TSState, c: Acceptor, a: Acceptor)
   requires type_ok(s) && type_ok(s') && valid(s) && c in leaders && a in acceptors
 {
     && s.leader_ballot[c] != -1 // leader n already has a ballot
-    //&& s.acceptor_state[a].highest != -1 // acceptor a may have agreed on some ballot value if highest == -1
-    && s.acceptor_state[a].highest < s.leader_ballot[c] // acceptor a has accepted some value for a lower ballot, or never promised a ballot
+    && s.acceptor_state[a].highest < s.leader_ballot[c] // acceptor a has not yet promised a ballot >= c's ballot
     // acceptor a promises with a message that contains c's ballot number
-    && s'.amsgs == s.amsgs + {AMsg(s.leader_ballot[c], s.acceptor_state[a].highest, s.acceptor_state[a].value, a)}
-    // acceptor a updates its highest (ballot, value) pair received so far --- // no need to update acceptor state 
-    //&& s'.acceptor_state == s.acceptor_state[a:= AState(s.leader_ballot[c], s.acceptor_state[a].value)]
-    && s'.acceptor_state == s.acceptor_state
+    && s'.pmsgs == s.pmsgs + {PMsg(s.leader_ballot[c], s.acceptor_state[a].highest, s.acceptor_state[a].value, a)}
+    // acceptor a updates its highest (ballot, value) pair received so far --- 
+    && s'.acceptor_state == s.acceptor_state[a := AState(s.leader_ballot[c], s.acceptor_state[a].value)]
     // all the other state components remain the same
     && s'.leader_ballot == s.leader_ballot
     && s'.leader_propose == s.leader_propose
     && s'.leader_decision == s.leader_decision
     && s'.ballot == s.ballot
     && s'.cmsgs == s.cmsgs
-    && s'.empty_count == s.empty_count
-    && s'.ballot_count == s.ballot_count
+    && s'.promise_count == s.promise_count
     && s'.decision_count == s.decision_count
 }
 
-// Before step 2a: message received by a leader (copied from amsg)
+// Before step 2a: message received by a leader (copied from pmsg)
 ghost predicate receive_response_1b(s: TSState, s': TSState, c: Acceptor, a: Acceptor, bn: int, highest: int, value: Proposal)
   requires type_ok(s) && type_ok(s') && valid(s) && c in leaders && a in acceptors
 {
-    && AMsg(bn, highest, value, a) in s.amsgs && s.leader_ballot[c] == bn
+    && PMsg(bn, highest, value, a) in s.pmsgs && s.leader_ballot[c] == bn
     && (
-      || (highest == -1 && s'.empty_count == s.empty_count[c:= s.empty_count[c]+{a}] 
-              && s'.ballot_count == s.ballot_count) // the empty_count case
-      || (highest != -1 && s'.ballot_count == s.ballot_count[c:= s.ballot_count[c]+{Promise(highest, value, a)}] 
-              && s'.empty_count == s.empty_count) // the ballot count case
-    ) // all the other state components remain the same
+      || (value != 0 && s'.leader_state == s.leader_state[c:= LState(s.leader_state[c].ballot, value)])
+      || (value == 0 && s'.leader_state == s.leader_state)
+    )
+    && s'.promise_count == s.promise_count[c:= s.promise_count[c]+{a}]
+    // all the other state components remain the same
     && s'.leader_ballot == s.leader_ballot
     && s'.leader_propose == s.leader_propose
     && s'.leader_decision == s.leader_decision
     && s'.ballot == s.ballot
     && s'.acceptor_state == s.acceptor_state
     && s'.decision_count == s.decision_count
-    && s'.amsgs == s.amsgs
+    && s'.pmsgs == s.pmsgs
     && s'.cmsgs == s.cmsgs
 }
 
@@ -181,10 +187,17 @@ ghost predicate receive_response_1b(s: TSState, s': TSState, c: Acceptor, a: Acc
 
 
 /* Why do we have consistency for Paxos? Intuitively, it could be understood in the following way.
-   If there is a ballot bn is observed to be decided with value v, there must be at least F + 1 acceptors promised 
-   that they will only reply to a ballot number greater than or equal to bn. Therefore, for all other ballot bn' < bn
-   those acceptors will not reply to any request with bn'; and for all new ballot bn'' >= bn, those acceptors will
-   reply with (bn'', bn, v) in Step 1b. Since the leader with bn'' is honest, he will be forced in Step 2a to propose v 
-   if it receives >(F + 1) Step 1b messages; he will not propose another value v' as there will be impossible for it
-   to receive >(F + 1) Step 1b message for a different value.
+   If there is a ballot bn that is observed as having been decided with value v, then
+   (1) there must be at least F + 1 acceptors promised in Step 1b that they will only reply to a ballot number greater than or equal to bn, and
+   (2) the same F+1 acceptors have sent out a confirm reply in Step 2b in response to the proposer with ballot number bn for v. 
+   
+   Therefore, for all other ballots bn' < bn those acceptors will not reply to any request with bn'; and for all new ballot bn'' >= bn, 
+   those acceptors will reply with (bn'', bn, v) in Step 1b since they have previously confirmed that value. 
+   (Note they cannot all go faulty which is against our assumption) Since the leader with bn'' is honest, 
+   he will be forced in Step 2a to propose v (with bn'') if it receives at least one Step 1b message with a confirmed v; 
+   He will not propose a different value unless it has not received any Step 1b message with a confirmed v 
+   (Intuitively, that value "v" should have already been confirmed by the system but it may still be waiting 
+   for a proposer to "announce" that it is confirmed).
+
+   In general, we cannot distinguish the case when a user is faulty and the case that a message from or to that user is taking too long. 
  */
